
### Geometric Series up to n
$$
\begin{align}
S_n&=\sum\limits_{i=0}^{n-1}a^ix
\\\\
S_n&=a^0x+a^1x+a^2x+\cdots+a^{n-1}x
\\\\
aS_n&=a^1x+a^2x+a^3x+\cdots+a^{n}x
\\\\
S_n-aS_n&=x-a^{n}x
\\\\\
S_n-aS_n&=x(1-a^n)
\\\\\
S_n(1-a)&=x(1-a^n)
\\\\\
S_n&=x\dfrac{(1-a^n)}{1-a}
\end{align}
$$
### Geometric series up to $\infty$
Using the proof for $S_n$ we can calculate the limit of $S$ when $n$ approaches $\infty$

If $a < 1$ then the limit converges and we can find a definite value. Otherwise the limit diverges to negative infinity

$$
\begin{align}
\lim\limits_{n\rightarrow\infty}x\dfrac{1-a^n}{1-a}&=\dfrac{x}{1-a},~~&a<1
\\\\
\lim\limits_{n\rightarrow\infty}x\dfrac{1-a^n}{1-a}&=0 &a=1
\\\\
\lim\limits_{n\rightarrow\infty}x\dfrac{1-a^n}{1-a}&=\infty, &a>1
\end{align}
$$
